DeBruijnSSA/BinSyntax/Typing/Term/Structural.lean
@@ -10,7 +10,7 @@ section Product
 
 variable
   [Φ: EffInstSet φ (Ty α) ε] [PartialOrder α] [SemilatticeSup ε] [OrderBot ε]
-  {Γ Δ : Ctx α ε} {σ : Region.Subst φ}
+  {Γ Δ : Ctx α ε}
 
 def pack : ℕ → Term φ
   | 0 => unit
@@ -56,38 +56,42 @@ theorem InS.wk_eff_pack {Γ : Ctx α ε} {h : ∀i, Γ.effect i ≤ lo} {h' : lo
   : (pack (φ := φ) h).wk_eff h' = pack (λi => (h i).trans h') := by
   ext; simp
 
-def unpack0 (x : ℕ) : Term φ := pl (pr^[x] (var 0))
+def pi_n (x : ℕ) (e : Term φ) : Term φ :=  pl (pr^[x] e)
+
+-- TODO: pi_n well-formedness lore
+
+def proj_n (x : ℕ) : Term φ := pl (pr^[x] (var 0))
 
 @[simp]
-theorem wk_lift_unpack0 {x : ℕ} : (unpack0 (φ := φ) x).wk (Nat.liftWk ρ) = unpack0 x := by
-  simp only [unpack0, wk_pl]
+theorem wk_lift_proj_n {x : ℕ} : (proj_n (φ := φ) x).wk (Nat.liftWk ρ) = proj_n x := by
+  simp only [proj_n, wk_pl]
   apply congrArg
   induction x with
   | zero => rfl
   | succ x ih => simp only [wk_pr, Function.iterate_succ_apply', ih]
 
 @[simp]
-theorem fvi_unpack0 {x : ℕ} : fvi (unpack0 (φ := φ) x) = 1 := by
+theorem fvi_proj_n {x : ℕ} : fvi (proj_n (φ := φ) x) = 1 := by
   simp only [fvi, Nat.reduceAdd, le_refl, tsub_eq_zero_of_le, zero_le, max_eq_left]
   induction x with
   | zero => rfl
   | succ x ih => simp [Function.iterate_succ_apply', ih]
 
 @[simp]
-theorem subst_lift_unpack0 {x : ℕ} {σ : Subst φ} : (unpack0 x).subst σ.lift = unpack0 x := by
-  simp only [unpack0, subst_pl]
+theorem subst_lift_proj_n {x : ℕ} {σ : Subst φ} : (proj_n x).subst σ.lift = proj_n x := by
+  simp only [proj_n, subst_pl]
   apply congrArg
   induction x with
   | zero => rfl
   | succ x ih => simp only [subst_pr, Function.iterate_succ_apply', ih]
 
 @[simp]
-theorem wk1_unpack0 {x : ℕ} : (unpack0 (φ := φ) x).wk1 = unpack0 x := wk_lift_unpack0
+theorem wk1_proj_n {x : ℕ} : (proj_n (φ := φ) x).wk1 = proj_n x := wk_lift_proj_n
 
 @[simp]
-theorem subst0_nil_pr_unpack0 {x : ℕ} : (unpack0 x).subst nil.pr.subst0 = unpack0 (φ := φ) (x + 1)
+theorem subst0_nil_pr_proj_n {x : ℕ} : (proj_n x).subst nil.pr.subst0 = proj_n (φ := φ) (x + 1)
   := by
-  simp only [unpack0, subst_pl]
+  simp only [proj_n, subst_pl]
   apply congrArg
   induction x with
   | zero => rfl
@@ -99,11 +103,11 @@ theorem Wf.pack_drop' {Γ Δ : Ctx α ε} {i : ℕ} (hi : i < Γ.length)
   := by induction i generalizing Γ with
   | zero => cases Γ with
     | nil => cases hi
-    | cons _ Γ => simp [unpack0, Ctx.pack]
+    | cons _ Γ => simp [proj_n, Ctx.pack]
   | succ i I => cases Γ with
     | nil => cases hi
     | cons head Γ =>
-      simp only [BinSyntax.Term.unpack0, List.length_cons, Fin.val_succ, Function.iterate_succ',
+      simp only [BinSyntax.Term.proj_n, List.length_cons, Fin.val_succ, Function.iterate_succ',
         Function.comp_apply, List.get_eq_getElem, List.getElem_cons_succ, Ctx.pack]
       apply Wf.pr
       convert I (Γ := head::Γ) (Nat.lt_of_succ_lt hi)
@@ -126,8 +130,8 @@ theorem Wf.pack_drop {Γ Δ : Ctx α ε} {i : ℕ} (hi : i < Γ.length)
   : Wf (φ := φ) ((Γ.pack, ⊥)::Δ) (Term.pr^[i] (Term.var 0)) (Ctx.pack (Γ.drop i), e)
   := by rw [Ctx.pack_drop hi]; apply Wf.pack_drop' hi
 
-theorem Wf.unpack0 {Γ Δ : Ctx α ε} {i : Fin Γ.length}
-  : Wf (φ := φ) ((Γ.pack, ⊥)::Δ) (unpack0 i) ((Γ.get i).1, e)
+theorem Wf.proj_n {Γ Δ : Ctx α ε} {i : Fin Γ.length}
+  : Wf (φ := φ) ((Γ.pack, ⊥)::Δ) (proj_n i) ((Γ.get i).1, e)
   := Wf.pl (pack_drop' i.prop)
 
 def InS.pack_drop {Γ Δ : Ctx α ε} (i : Fin Γ.length)
@@ -164,46 +168,46 @@ def InS.pack_drop_succ {Γ Δ : Ctx α ε} (i : Fin Γ.length)
   rw [<-Term.pr, <-Function.iterate_succ_apply, Function.iterate_succ_apply']
   rfl
 
-def InS.unpack0 {Γ Δ : Ctx α ε} (i : Fin Γ.length)
+def InS.proj_n {Γ Δ : Ctx α ε} (i : Fin Γ.length)
   : InS φ ((Γ.pack, ⊥)::Δ) ((Γ.get i).1, e)
-  := ⟨Term.unpack0 i, Wf.unpack0⟩
+  := ⟨Term.proj_n i, Wf.proj_n⟩
 
 theorem InS.pl_pack_drop' {Γ Δ : Ctx α ε} {i : Fin Γ.length}
-  : (InS.pack_drop' (φ := φ) (Δ := Δ) (e := e) i).pl = unpack0 i := rfl
+  : (InS.pack_drop' (φ := φ) (Δ := Δ) (e := e) i).pl = proj_n i := rfl
 
-theorem InS.coe_unpack0 {Γ Δ : Ctx α ε} {i : Fin Γ.length}
-  : (InS.unpack0 (φ := φ) (Δ := Δ) (e := e) i : Term φ) = Term.unpack0 i := rfl
+theorem InS.coe_proj_n {Γ Δ : Ctx α ε} {i : Fin Γ.length}
+  : (InS.proj_n (φ := φ) (Δ := Δ) (e := e) i : Term φ) = Term.proj_n i := rfl
 
--- TODO: wk_lift unpack0
+-- TODO: wk_lift proj_n
 
--- TODO: subst_lift unpack0
-
-@[simp]
-theorem InS.wk1_unpack0 {Γ Δ : Ctx α ε} {i : Fin Γ.length}
-  : (InS.unpack0 (φ := φ) (Γ := Γ) (Δ := Δ) (e := e) i).wk1 (inserted := inserted) = unpack0 i := by
-  ext; rw [coe_unpack0, coe_wk1, coe_unpack0, Term.wk1_unpack0]
+-- TODO: subst_lift proj_n
 
 @[simp]
-theorem InS.wk_lift_unpack0 {Γ Δ : Ctx α ε} {i : Fin Γ.length} {ρ : Γ.InS Δ}
-  : (InS.unpack0 (φ := φ) (Γ := Γ) (Δ := Δ) (e := e) i).wk (ρ.lift (le_refl _)) = unpack0 i := by
-  ext; rw [coe_unpack0, coe_wk, coe_unpack0, Ctx.InS.coe_lift, Term.wk_lift_unpack0]
+theorem InS.wk1_proj_n {Γ Δ : Ctx α ε} {i : Fin Γ.length}
+  : (InS.proj_n (φ := φ) (Γ := Γ) (Δ := Δ) (e := e) i).wk1 (inserted := inserted) = proj_n i := by
+  ext; rw [coe_proj_n, coe_wk1, coe_proj_n, Term.wk1_proj_n]
 
 @[simp]
-theorem InS.subst_lift_unpack0 {Γ Δ Δ' : Ctx α ε} {i : Fin Γ.length} {σ : Subst.InS φ Δ' Δ}
-  : (InS.unpack0 (φ := φ) (Γ := Γ) (Δ := Δ) (e := e) i).subst (σ.lift (le_refl _)) = unpack0 i := by
-  ext; rw [coe_unpack0, coe_subst, coe_unpack0, Subst.InS.coe_lift, Term.subst_lift_unpack0]
+theorem InS.wk_lift_proj_n {Γ Δ : Ctx α ε} {i : Fin Γ.length} {ρ : Γ.InS Δ}
+  : (InS.proj_n (φ := φ) (Γ := Γ) (Δ := Δ) (e := e) i).wk (ρ.lift (le_refl _)) = proj_n i := by
+  ext; rw [coe_proj_n, coe_wk, coe_proj_n, Ctx.InS.coe_lift, Term.wk_lift_proj_n]
 
 @[simp]
-theorem InS.subst0_nil_pr_unpack0 {Γ Δ : Ctx α ε} {i : Fin Γ.length}
-  : (InS.unpack0 (φ := φ) (Γ := Γ) (e := e) i).subst (nil.pr.subst0)
-  = unpack0 (φ := φ) (Γ := V::Γ) (Δ := Δ) i.succ := by ext; exact Term.subst0_nil_pr_unpack0
+theorem InS.subst_lift_proj_n {Γ Δ Δ' : Ctx α ε} {i : Fin Γ.length} {σ : Subst.InS φ Δ' Δ}
+  : (InS.proj_n (φ := φ) (Γ := Γ) (Δ := Δ) (e := e) i).subst (σ.lift (le_refl _)) = proj_n i := by
+  ext; rw [coe_proj_n, coe_subst, coe_proj_n, Subst.InS.coe_lift, Term.subst_lift_proj_n]
 
-def unpack0' (n : ℕ) (i : ℕ) : Term φ := match n with
+@[simp]
+theorem InS.subst0_nil_pr_proj_n {Γ Δ : Ctx α ε} {i : Fin Γ.length}
+  : (InS.proj_n (φ := φ) (Γ := Γ) (e := e) i).subst (nil.pr.subst0)
+  = proj_n (φ := φ) (Γ := V::Γ) (Δ := Δ) i.succ := by ext; exact Term.subst0_nil_pr_proj_n
+
+def proj_n' (n : ℕ) (i : ℕ) : Term φ := match n with
 | 0 => unit
-| n + 1 => let2 (var 0) (match i with | 0 => var 1 | i + 1 => unpack0' n i)
+| n + 1 => let2 (var 0) (match i with | 0 => var 1 | i + 1 => proj_n' n i)
 
-theorem Wf.unpack0' {Γ Δ : Ctx α ε} (i : Fin Γ.length)
-  : Wf (φ := φ) ((Γ.pack, ⊥)::Δ) (unpack0' Γ.length i) ((Γ.get i).1, e)
+theorem Wf.proj_n' {Γ Δ : Ctx α ε} (i : Fin Γ.length)
+  : Wf (φ := φ) ((Γ.pack, ⊥)::Δ) (proj_n' Γ.length i) ((Γ.get i).1, e)
   := by induction Γ generalizing Δ with
   | nil => exact i.elim0
   | cons V Γ I =>
@@ -215,41 +219,41 @@ theorem Wf.unpack0' {Γ Δ : Ctx α ε} (i : Fin Γ.length)
       simp only [List.length_cons, Fin.val_succ, List.get_eq_getElem, List.getElem_cons_succ]
       exact I i
 
-def InS.unpack0' {Γ Δ : Ctx α ε} (i : Fin Γ.length) : InS φ ((Γ.pack, ⊥)::Δ) ((Γ.get i).1, e)
+def InS.proj_n' {Γ Δ : Ctx α ε} (i : Fin Γ.length) : InS φ ((Γ.pack, ⊥)::Δ) ((Γ.get i).1, e)
   := match Γ with
   | [] => i.elim0
   | V::Γ => let2
     (var (V := (V.1.prod (Ctx.pack Γ), e)) 0 (by simp [Ctx.pack]))
-    (i.cases (var 1 (by simp)) (λi => unpack0' (Γ := Γ) i))
+    (i.cases (var 1 (by simp)) (λi => proj_n' (Γ := Γ) i))
 
 @[simp]
-theorem InS.coe_unpack0' {Γ Δ : Ctx α ε} {i : Fin Γ.length}
-  : (InS.unpack0' (φ := φ) (Δ := Δ) (e := e) i : Term φ) = Term.unpack0' Γ.length i := by
+theorem InS.coe_proj_n' {Γ Δ : Ctx α ε} {i : Fin Γ.length}
+  : (InS.proj_n' (φ := φ) (Δ := Δ) (e := e) i : Term φ) = Term.proj_n' Γ.length i := by
   induction Γ generalizing Δ with
   | nil => exact i.elim0
   | cons V Γ I =>
-    simp only [List.get_eq_getElem, List.length_cons, Set.mem_setOf_eq, unpack0', Fin.val_zero,
-      List.getElem_cons_zero, InS.coe_let2, coe_var, Term.unpack0', let2.injEq, true_and]
+    simp only [List.get_eq_getElem, List.length_cons, Set.mem_setOf_eq, proj_n', Fin.val_zero,
+      List.getElem_cons_zero, InS.coe_let2, coe_var, Term.proj_n', let2.injEq, true_and]
     cases i using Fin.cases with
     | zero => rfl
     | succ i => exact I
 
-theorem InS.unpack0_zero' {Γ Δ : Ctx α ε}
-  : InS.unpack0' (φ := φ) (Γ := V::Γ) (Δ := Δ) (e := e) (by simp only [List.length_cons]; exact 0)
+theorem InS.proj_n_zero' {Γ Δ : Ctx α ε}
+  : InS.proj_n' (φ := φ) (Γ := V::Γ) (Δ := Δ) (e := e) (by simp only [List.length_cons]; exact 0)
   = (by simp only [Ctx.pack]; apply InS.pi_l) := rfl
 
-theorem InS.unpack0_succ' {Γ Δ : Ctx α ε} {i : Fin Γ.length}
-  : InS.unpack0' (φ := φ) (Γ := V::Γ) (Δ := Δ) (e := e) i.succ
+theorem InS.proj_n_succ' {Γ Δ : Ctx α ε} {i : Fin Γ.length}
+  : InS.proj_n' (φ := φ) (Γ := V::Γ) (Δ := Δ) (e := e) i.succ
   = let2
     (var (V := (V.1.prod (Ctx.pack Γ), e)) 0 (by simp [Ctx.pack]))
-    (unpack0' (Γ := Γ) i) := rfl
+    (proj_n' (Γ := Γ) i) := rfl
 
-def Subst.unpack0 : Subst φ := λi => Term.unpack0 i
+def Subst.proj_n : Subst φ := λi => Term.proj_n i
 
-theorem Subst.Wf.unpack0 {Γ Δ : Ctx α ε}
-  : Subst.Wf (φ := φ) ((Γ.pack, ⊥)::Δ) Γ Subst.unpack0 := λ_ => Term.Wf.unpack0
+theorem Subst.Wf.proj_n {Γ Δ : Ctx α ε}
+  : Subst.Wf (φ := φ) ((Γ.pack, ⊥)::Δ) Γ Subst.proj_n := λ_ => Term.Wf.proj_n
 
-def Subst.InS.unpack {Γ Δ : Ctx α ε} : Subst.InS φ ((Γ.pack, ⊥)::Δ) Γ := ⟨Subst.unpack0, Wf.unpack0⟩
+def Subst.InS.unpack {Γ Δ : Ctx α ε} : Subst.InS φ ((Γ.pack, ⊥)::Δ) Γ := ⟨Subst.proj_n, Wf.proj_n⟩
 
 def Subst.pack (n : ℕ) : Subst φ := λ_ => Term.pack n
 
@@ -275,67 +279,117 @@ section Sum
 
 variable
   [Φ: EffInstSet φ (Ty α) ε] [PartialOrder α] [PartialOrder ε] [OrderBot ε]
-  {Γ Δ : Ctx α ε} {σ : Region.Subst φ}
+  {Γ Δ : Ctx α ε}
 
-def pack0 (ℓ : ℕ) : Term φ := inr^[ℓ] (inl (var 0))
+def inj (ℓ : ℕ) (e : Term φ) : Term φ := inr^[ℓ] (inl e)
 
 @[simp]
-theorem wk_lift_pack0 {ℓ : ℕ} : (pack0 ℓ).wk (Nat.liftWk ρ) = pack0 (φ := φ) ℓ := by
-  simp only [pack0]
+theorem wk_inj {ℓ : ℕ} {e : Term φ} : (inj ℓ e).wk ρ = inj ℓ (e.wk ρ) := by
+  simp only [inj]
   induction ℓ with
   | zero => rfl
   | succ ℓ ih => simp [ih, -Function.iterate_succ, Function.iterate_succ']
 
 @[simp]
-theorem wk1_pack0 : (pack0 ℓ).wk1 = pack0 (φ := φ) ℓ := by
-  simp only [wk1, wk_lift_pack0]
+theorem wk0_inj {ℓ : ℕ} {e : Term φ} : (inj ℓ e).wk0 = inj ℓ (e.wk0) := by
+  simp only [wk0, wk_inj]
 
 @[simp]
-theorem subst_lift_pack0 {ℓ : ℕ} {σ : Subst φ} : (pack0 ℓ).subst σ.lift = pack0 (φ := φ) ℓ := by
-  simp only [pack0]
+theorem wk1_inj {ℓ : ℕ} {e : Term φ} : (inj ℓ e).wk1 = inj ℓ (e.wk1) := by
+  simp only [wk1, wk_inj]
+
+@[simp]
+theorem wk2_inj {ℓ : ℕ} {e : Term φ} : (inj ℓ e).wk2 = inj ℓ (e.wk2) := by
+  simp only [wk2, wk_inj]
+
+@[simp]
+theorem subst_inj {ℓ : ℕ} {e : Term φ} : (inj ℓ e).subst σ = inj ℓ (e.subst σ) := by
+  simp only [inj]
   induction ℓ with
   | zero => rfl
   | succ ℓ ih => simp [ih, -Function.iterate_succ, Function.iterate_succ']
 
+theorem Wf.inj {Γ : Ctx α ε} {R : LCtx α} {i : Fin R.length} {a : Term φ}
+  (h : a.Wf Γ (R.get i, e)) : Term.Wf (φ := φ) Γ (inj i a) (R.pack, e)  := by
+  induction R generalizing Γ with
+  | nil => exact i.elim0
+  | cons _ _ I =>
+    cases i using Fin.cases with
+    | zero => exact Wf.inl $ h
+    | succ i =>
+      simp only [
+        Fin.val_succ, Function.iterate_succ', Function.comp_apply, LCtx.pack,
+        Wf.inr_iff, BinSyntax.Term.inj
+      ]
+      apply I
+      apply h
+
+def InS.inj {Γ : Ctx α ε} {R : LCtx α} {i : Fin R.length} (a : Term.InS φ Γ (R.get i, e))
+  : Term.InS φ Γ (R.pack, e) := ⟨a.val.inj i, a.prop.inj⟩
+
 @[simp]
-theorem Wf.pack0 {Γ : Ctx α ε} {R : LCtx α} {i : Fin R.length}
-  : Term.Wf (φ := φ) ((R.get i, ⊥)::Γ) (pack0 i) (R.pack, ⊥)  := by
+theorem InS.coe_inj {Γ : Ctx α ε} {R : LCtx α} {i : Fin R.length} {a : Term.InS φ Γ (R.get i, e)}
+  : (InS.inj (φ := φ) (Γ := Γ) (R := R) a : Term φ) = Term.inj i a := rfl
+
+def inj_n (ℓ : ℕ) : Term φ := inj ℓ nil
+
+@[simp]
+theorem wk_lift_inj_n {ℓ : ℕ} : (inj_n ℓ).wk (Nat.liftWk ρ) = inj_n (φ := φ) ℓ := by
+  simp only [inj_n, wk_inj, wk, Nat.liftWk_zero]; rfl
+
+@[simp]
+theorem wk1_inj_n : (inj_n ℓ).wk1 = inj_n (φ := φ) ℓ := by
+  simp only [wk1, wk_lift_inj_n]
+
+@[simp]
+theorem wk2_inj_n : (inj_n ℓ).wk2 = inj_n (φ := φ) ℓ := by
+  simp only [inj_n, wk2_inj]; rfl
+
+@[simp]
+theorem subst_lift_inj_n {ℓ : ℕ} {σ : Subst φ} : (inj_n ℓ).subst σ.lift = inj_n (φ := φ) ℓ := by
+  simp only [inj_n, subst_inj, subst, Subst.lift_zero]; rfl
+
+@[simp]
+theorem Wf.inj_n {Γ : Ctx α ε} {R : LCtx α} {i : Fin R.length}
+  : Term.Wf (φ := φ) ((R.get i, ⊥)::Γ) (inj_n i) (R.pack, ⊥)  := by
   induction R generalizing Γ with
   | nil => exact i.elim0
   | cons _ _ I =>
     cases i using Fin.cases with
     | zero => exact Wf.inl $ Wf.var Ctx.Var.shead
     | succ i =>
-      simp only [Fin.val_succ,
-        BinSyntax.Term.pack0, Function.iterate_succ', Function.comp_apply, LCtx.pack, Wf.inr_iff]
+      simp only [
+        Fin.val_succ, BinSyntax.Term.inj_n, Function.iterate_succ', Function.comp_apply, LCtx.pack,
+        Wf.inr_iff, BinSyntax.Term.inj
+      ]
       apply I
 
-def InS.pack0 {Γ : Ctx α ε} (R : LCtx α) (i : Fin R.length)
+def InS.inj_n {Γ : Ctx α ε} (R : LCtx α) (i : Fin R.length)
   : Term.InS φ ((R.get i, ⊥)::Γ) (R.pack, ⊥) :=
-  ⟨Term.pack0 i, Term.Wf.pack0⟩
+  ⟨Term.inj_n i, Term.Wf.inj_n⟩
 
 @[simp]
-theorem InS.coe_pack0 {Γ : Ctx α ε} {R : LCtx α} {i : Fin R.length}
-  : (InS.pack0 (φ := φ) (Γ := Γ) (R := R) i : Term φ) = Term.pack0 i := rfl
+theorem InS.coe_inj_n {Γ : Ctx α ε} {R : LCtx α} {i : Fin R.length}
+  : (InS.inj_n (φ := φ) (Γ := Γ) (R := R) i : Term φ) = Term.inj_n i := rfl
 
 @[simp]
-theorem InS.wk_lift_pack0 {Γ : Ctx α ε} {R : LCtx α} {i : Fin R.length} {ρ : Γ.InS Δ}
-  : (InS.pack0 (φ := φ) R i).wk (ρ.lift (le_refl _)) = pack0 R i := by ext; simp
+theorem InS.wk_lift_inj_n {Γ : Ctx α ε} {R : LCtx α} {i : Fin R.length} {ρ : Γ.InS Δ}
+  : (InS.inj_n (φ := φ) R i).wk (ρ.lift (le_refl _)) = inj_n R i := by ext; simp
 
 @[simp]
-theorem InS.wk_slift_pack0 {Γ : Ctx α ε} {R : LCtx α} {i : Fin R.length} {ρ : Γ.InS Δ}
-  : (InS.pack0 (φ := φ) R i).wk (ρ.slift) = pack0 R i := by ext; simp
+theorem InS.wk_slift_inj_n {Γ : Ctx α ε} {R : LCtx α} {i : Fin R.length} {ρ : Γ.InS Δ}
+  : (InS.inj_n (φ := φ) R i).wk (ρ.slift) = inj_n R i := by ext; simp
 
 @[simp]
-theorem InS.subst_lift_pack0 {Γ : Ctx α ε} {R : LCtx α} {i : Fin R.length} {σ : Subst.InS φ Γ Δ}
-  : (InS.pack0 (φ := φ) R i).subst (σ.lift (le_refl _)) = pack0 R i := by ext; simp
+theorem InS.subst_lift_inj_n {Γ : Ctx α ε} {R : LCtx α} {i : Fin R.length} {σ : Subst.InS φ Γ Δ}
+  : (InS.inj_n (φ := φ) R i).subst (σ.lift (le_refl _)) = inj_n R i := by ext; simp
 
 @[simp]
-theorem InS.subst_slift_pack0 {Γ : Ctx α ε} {R : LCtx α} {i : Fin R.length} {σ : Subst.InS φ Γ Δ}
-  : (InS.pack0 (φ := φ) R i).subst σ.slift = pack0 R i := by ext; simp
+theorem InS.subst_slift_inj_n {Γ : Ctx α ε} {R : LCtx α} {i : Fin R.length} {σ : Subst.InS φ Γ Δ}
+  : (InS.inj_n (φ := φ) R i).subst σ.slift = inj_n R i := by ext; simp
 
 @[simp]
-theorem InS.wk1_pack0 {Γ : Ctx α ε} {R : LCtx α} {i : Fin R.length}
-  : (InS.pack0 (φ := φ) (Γ := Γ) R i).wk1 (inserted := inserted) = pack0 R i := by ext; simp
+theorem InS.wk1_inj_n {Γ : Ctx α ε} {R : LCtx α} {i : Fin R.length}
+  : (InS.inj_n (φ := φ) (Γ := Γ) R i).wk1 (inserted := inserted) = inj_n R i := by ext; simp
 
 end Sum
