DeBruijnSSA/BinSyntax/Rewrite/Region/Compose/Structural/Basic.lean
@@ -1,0 +1,24 @@
+import DeBruijnSSA.BinSyntax.Rewrite.Region.Compose.Structural.Sum
+import DeBruijnSSA.BinSyntax.Rewrite.Region.Compose.Structural.Product
+
+namespace BinSyntax
+
+variable [Φ: EffInstSet φ (Ty α) ε] [PartialOrder α] [SemilatticeSup ε] [OrderBot ε]
+
+namespace Region
+
+def Eqv.packed {Γ : Ctx α ε} {R : LCtx α} (r : Eqv φ Γ R) : Eqv φ [(Γ.pack, ⊥)] [R.pack]
+  := r.packed_out.packed_in
+
+def Eqv.unpacked {Γ : Ctx α ε} {R : LCtx α} (r : Eqv φ [(Γ.pack, ⊥)] [R.pack]) (h : Γ.Pure)
+  : Eqv φ Γ R := r.unpacked_out.unpacked_in h
+
+-- TODO: (un)packed_in commutes with (un)packed_out
+
+-- TODO: packed_unpacked, unpacked_packed
+
+-- TODO: {br, let1, let2, case, cfg}
+
+end Region
+
+end BinSyntax
