DeBruijnSSA/BinSyntax/Rewrite/Term/Compose/Structural/Sum.lean
@@ -1,0 +1,58 @@
+import DeBruijnSSA.BinSyntax.Rewrite.Term.Compose.Seq
+import DeBruijnSSA.BinSyntax.Rewrite.Term.Compose.Sum
+import DeBruijnSSA.BinSyntax.Rewrite.Term.Compose.Product
+import DeBruijnSSA.BinSyntax.Typing.Term.Structural
+
+
+namespace BinSyntax
+
+variable [Φ: EffInstSet φ (Ty α) ε] [PartialOrder α] [SemilatticeSup ε] [OrderBot ε]
+
+namespace Term
+
+set_option linter.unusedVariables false in
+def Eqv.inj
+  {Γ : Ctx α ε} {R : LCtx α} {i : Fin R.length} (a : Eqv φ Γ (R.get i, e)) : Eqv φ Γ (R.pack, e)
+  := match R with
+  | [] => i.elim0
+  | _::R => by cases i using Fin.cases with | zero => exact a.inl | succ i => exact inr (inj a)
+
+-- TODO: pack_inj is just inj (nil)
+
+def Eqv.inj_n {Γ : Ctx α ε} (R : LCtx α) (i : Fin R.length) : Eqv φ ((R.get i, ⊥)::Γ) (R.pack, e)
+  := match R with
+  | [] => i.elim0
+  | _::R => i.cases (inl nil) (λi => inr (inj_n R i))
+
+theorem Eqv.inj_n_def {Γ : Ctx α ε} {R : LCtx α} {i : Fin R.length}
+  : Eqv.inj_n (φ := φ) (Γ := Γ) R i = ⟦Term.InS.inj_n R i⟧ := by
+  induction R generalizing Γ with
+  | nil => exact i.elim0
+  | cons _ _ I =>
+    cases i using Fin.cases with
+    | zero => rfl
+    | succ i =>
+      simp only [inj_n, I, inr_quot, Fin.cases_succ]
+      apply congrArg
+      ext
+      simp [Term.inj_n, Term.inj, Term.Wf.inj_n, -Function.iterate_succ, Function.iterate_succ']
+
+-- def Eqv.pack_case {Γ : Ctx α ε} {R : LCtx α}
+--   (d : Eqv φ Γ (R.pack, e)) (G : ∀i : Fin R.length, Eqv φ ((R.get i, ⊥)::Γ) (A, e))
+--   : Eqv φ Γ (C, e) := sorry
+
+-- def Eqv.pack_app_inl {Γ : Ctx α ε} {L R : LCtx α} : Eqv φ ((L.pack, ⊥)::Γ) ((L ++ R).pack, e)
+--   := sorry
+
+-- def Eqv.pack_app_inr {Γ : Ctx α ε} {L R : LCtx α} : Eqv φ ((R.pack, ⊥)::Γ) ((L ++ R).pack, e)
+--   := sorry
+
+-- def Eqv.pack_app {Γ : Ctx α ε} {L R : LCtx α}
+--   : Eqv φ (((L ++ R).pack, ⊥)::Γ) (L.pack.coprod R.pack, e)
+--   := sorry
+
+-- TODO: pack_app
+
+-- TODO: pack_app_pack_case => pack_case
+
+end Term
